$$
\begin{aligned}
    w(r_0)&=\frac{r_{0}}{\sqrt{r(2 r_{0}-r)}}\left[1-\frac{a_{T} r_{0}^{2}}{\mu}\left(3 \sin ^{-1}(\sqrt{\frac{r}{2 r_{0}}})-\frac{3 \pi}{4}+2\right)\right]+\frac{a_{T} r_{0}}{2 \mu}(r+3 r_{0})_{{\huge|}_{\small{r=r_0}}}\\
    &= \frac{r_{0}}{\sqrt{r_0^2}}\left[1-\frac{a_{T} r_{0}^{2}}{\mu}\left(3 \sin ^{-1}(\sqrt{\frac{1}{2}})-\frac{3 \pi}{4}+2\right)\right]+\frac{a_{T} r_{0}}{2 \mu}(4r_{0})\\
    &= 1-\frac{a_{T} r_{0}^{2}}{\mu}\left(\frac{3\pi}{4}-\frac{3 \pi}{4}+2\right)+\frac{a_{T} r_{0}}{2 \mu}(4r_{0})\\
    &= 1-\frac{2a_{T} r_{0}^{2}}{\mu}+\frac{2a_{T} r_{0}^2}{\mu}=1\\

    w(2r_0)&=\lim_{r\to 2r_0}\left[\frac{r_{0}}{\sqrt{r(2 r_{0}-r)}}\left[1-\frac{a_{T} r_{0}^{2}}{\mu}\left(3 \sin ^{-1}(\sqrt{\frac{r}{2 r_{0}}})-\frac{3 \pi}{4}+2\right)\right]+\frac{a_{T} r_{0}}{2 \mu}(r+3 r_{0})\right]\\
    &= \lim_{r\to 2r_0}\frac{r_{0}}{\sqrt{r(2 r_{0}-r)}}\lim_{r\to 2r_0}\left[1-\frac{a_{T} r_{0}^{2}}{\mu}\left(3 \sin ^{-1}(\sqrt{\frac{r}{2 r_{0}}})-\frac{3 \pi}{4}+2\right)\right] + \lim_{r\to 2r_0}\frac{a_{T} r_{0}}{2 \mu}(r+3 r_{0})\\
    &=\lim_{r\to 2r_0}\frac{r_{0}}{\sqrt{r(2 r_{0}-r)}}\left[1-\frac{a_{T} r_{0}^{2}}{\mu}\left(\frac{3\pi}{2}-\frac{3 \pi}{4}+2\right)\right]+\frac{5a_Tr_0^2}{2\mu}\\
    &= \lim_{r\to 2r_0}\frac{r_{0}}{\sqrt{r(2 r_{0}-r)}}\left[\frac{2\mu-(3\pi+4)a_{T} r_{0}^{2}}{2\mu}\right]+\frac{5a_Tr_0^2}{2\mu}\\
\end{aligned}
$$